src/TV/mtv_correct.v
@@ -18,13 +18,15 @@ Require Import trace.
 Require Import symexe_def.
 Require Import assoclist.
 Require Import ssa_props.
+Require Import sub_tv_def.
 Require Import sub_tv_dec.
 Require Import sub_tv_infer.
 Require Import sub_tv.
 Require Import Coq.Bool.Sumbool.
 Require Import symexe_tactic.
+Require Import sub_tv_correct.
 
-Definition ptr_has_basebound TD M vb ve vp : bool :=
+Definition mptr_has_basebound TD M vb ve vp : bool :=
 match (GV2ptr TD (getPointerSize TD) vb, 
        GV2ptr TD (getPointerSize TD) ve,
        GV2ptr TD (getPointerSize TD) vp) with
@@ -36,6 +38,14 @@ match (GV2ptr TD (getPointerSize TD) vb,
 | _ => false
 end.
 
+Definition fptr_has_basebound fs vb ve vp : bool :=
+match (lookupFdefViaGVFromFunTable fs vb,
+       lookupFdefViaGVFromFunTable fs ve,
+       lookupFdefViaGVFromFunTable fs vp) with
+| (Some fid1, Some fid2, Some fid3) => eq_id fid1 fid2 && eq_id fid3 fid3
+| _ => false
+end.        
+
 (* fs: function table
  * lc: local variable mappings
 *)
@@ -45,19 +55,13 @@ match md with
 | nil => true
 | (fid,lbl,nth,b,e,p,true)::md' =>
     match (lookupAL _ lc b, lookupAL _ lc e, lookupAL _ lc p) with
-    | (Some vb, Some ve, Some vp) => ptr_has_basebound TD M vb ve vp
+    | (Some vb, Some ve, Some vp) => mptr_has_basebound TD M vb ve vp
     | (None, None, None) => true
     | _ => false
     end && valid_metadata TD fs lc M md'
 | (fid,lbl,nth,b,e,p,false)::md' => 
     match (lookupAL _ lc b, lookupAL _ lc e, lookupAL _ lc p) with
-    | (Some vb, Some ve, Some vp) => 
-        match (lookupFdefViaGVFromFunTable fs vb,
-               lookupFdefViaGVFromFunTable fs ve,
-               lookupFdefViaGVFromFunTable fs vp) with
-        | (Some fid1, Some fid2, Some fid3) => eq_id fid1 fid2 && eq_id fid3 fid3
-        | _ => false
-        end        
+    | (Some vb, Some ve, Some vp) => fptr_has_basebound fs vb ve vp
     | (None, None, None) => true
     | _ => false
     end && valid_metadata TD fs lc M md'
@@ -69,19 +73,126 @@ Definition valid_memdata_db (TD:TargetData) (M:mem) :=
   mload TD M addrofp (typ_pointer t) Align.One = Some vp ->
   is_hashLoadBaseBound fid = true ->
   callLib M fid (params2GVs TD 
-    (p::
-     (typ_pointer (typ_pointer (typ_int Size.Eight)),vaddrofb)::
-     (typ_pointer (typ_pointer (typ_int Size.Eight)),vaddrofe)::
-     ps) lc gl) = 
-    Some (oresult, M') ->
+    (p::(SBsyntax.pp8,vaddrofb)::(SBsyntax.pp8,vaddrofe)::ps) lc gl) = 
+    Some (oresult, M', Rok) ->
   getOperandValue TD vaddrofb lc gl = Some addrofb ->
   getOperandValue TD vaddrofe lc gl = Some addrofe ->
   mload TD M' addrofb (typ_pointer (typ_int Size.Eight)) Align.One = Some vb ->
   mload TD M' addrofe (typ_pointer (typ_int Size.Eight)) Align.One = Some ve ->
-  ptr_has_basebound TD M vb ve vp = true.
+  mptr_has_basebound TD M vb ve vp = true.
 
+Definition flnbeps_to_metadata (md:flnbeps) : metadata :=
+List.fold_left (fun accum => fun flnbep => 
+  let '(fid, lnbep) := flnbep in
+  List.fold_left (fun accum => fun lnbep =>
+    let '(l1,nbep) := lnbep in
+    List.fold_left (fun accum => fun nbep =>
+      let '(n1,bep) := nbep in
+      List.fold_left (fun accum => fun elt =>
+        let '(b,e,p,flag) := elt in
+        (fid,l1,n1,b,e,p,flag)::accum
+        ) bep accum
+      ) nbep accum
+    ) lnbep accum
+  ) md nil.
+
+Lemma check_mptr_metadata__is__correct : forall Ps2 fid1 l1 i1 base bound ptr
+  TD lc gl Mem vb ve vp fs md m2 flnbep,
+  validate_metadata_from_module m2 flnbep = true ->
+  flnbeps_to_metadata flnbep = md ->
+  valid_metadata TD fs lc Mem md = true ->
+  valid_memdata_db TD Mem = true ->
+  check_mptr_metadata Ps2 fid1 l1 i1 base bound ptr = true ->
+  sterm_denotes_genericvalue TD lc gl Mem base vb ->
+  sterm_denotes_genericvalue TD lc gl Mem bound ve ->
+  sterm_denotes_genericvalue TD lc gl Mem ptr vp ->
+  mptr_has_basebound TD Mem vb ve vp = true.
+(* We need to say
+   1) il in l1 in fid1 in Ps1 in m1 <= Ps2 in m2
+*)
+Admitted.
+
+Lemma mptr_has_basebound__eq_ptr_object : forall TD lc gl Mem ptr ptr' vb ve vp 
+  vp',
+  sterm_denotes_genericvalue TD lc gl Mem (get_ptr_object ptr) vp ->
+  sterm_denotes_genericvalue TD lc gl Mem (get_ptr_object ptr') vp' ->
+  eq_sterm (get_ptr_object ptr) (get_ptr_object ptr') ->
+  mptr_has_basebound TD Mem vb ve vp = mptr_has_basebound TD Mem vb ve vp'.
+Admitted.
+
+Definition mptr_inbounds (TD:TargetData) M vb ve vp t : bool :=
+match (GV2ptr TD (getPointerSize TD) vb, 
+       GV2ptr TD (getPointerSize TD) ve,
+       GV2ptr TD (getPointerSize TD) vp) with
+| (Some (Vptr bb ob), Some (Vptr be oe), Some (Vptr bp op)) =>
+  match getTypeAllocSize TD t with
+  | None => false
+  | Some tsz =>
+    let '(lo,hi) := Memory.Mem.bounds M bp in
+    bzeq bb be && bzeq bb bp && 
+    Zle_bool (Integers.Int.unsigned 31 ob) (Integers.Int.unsigned 31 op) &&
+    Zle_bool (Integers.Int.unsigned 31 op) 
+             (Integers.Int.unsigned 31 oe + Size.to_Z tsz)
+  end
+| _ => false
+end.
+
+Definition pars_of_loadStoreDereferenceCheck t vp vb ve psafe :=
+((typ_pointer t,vp)::
+     (SBsyntax.p8,vb)::
+     (SBsyntax.p8,ve)::
+     (SBsyntax.i32,
+      (value_const 
+        (const_castop 
+          castop_ptrtoint
+          (const_gep false 
+            (const_null t) 
+            (Cons_list_const (const_int SBsyntax.sz32 1%Z) Nil_list_const)
+          )
+          SBsyntax.i32
+        )
+      )
+     )::(SBsyntax.i32,psafe)::nil).
+
+Axiom call_loadStoreDereferenceCheck : forall fid M TD t vp vb ve lc gl oresult
+  b e p psafe r,
+  is_loadStoreDereferenceCheck fid = true ->
+  callLib M fid (params2GVs TD 
+    (pars_of_loadStoreDereferenceCheck t vp vb ve psafe) lc gl) = 
+    Some (oresult, M, r) ->
+  getOperandValue TD vb lc gl = Some b ->
+  getOperandValue TD ve lc gl = Some e ->
+  getOperandValue TD vp lc gl = Some p ->
+  (mptr_inbounds (TD:TargetData) M b e p t = true <-> r = Rok).
   
+Lemma mtv_cmds_inv : forall Ps1 Ps2 fid l1 nbs2 cs2 id2 t2 v2 a2 TD lc gl ptr,
+  mtv_cmds Ps1 Ps2 fid l1 nbs2 = true ->
+  nbranchs2cmds nbs2 = cs2 ->
+  getOperandValue TD v2 lc gl = Some ptr ->
+  InCmdsB (insn_load id2 t2 v2 a2) cs2 -> 
+  exists cs21, exists cs22, exists cs23,
+  exists id1, exists nr1, exists tc1, exists rt1, exists ft, exists fid,
+  exists t, exists vp, exists vb, exists ve, exists psafe, 
+    cs2 = cs21 ++ 
+    [insn_call id1 nr1 tc1 rt1 (value_const (const_gid ft fid))
+      (pars_of_loadStoreDereferenceCheck t vp vb ve psafe)] ++ cs22 ++ 
+    [insn_load id2 t2 v2 a2]++ cs23 /\
+    is_loadStoreDereferenceCheck fid = true /\
+    getOperandValue TD vp lc gl = Some ptr. 
+Admitted.
 
+Lemma mtv_cmds__is__correct : forall Ps1 Ps2 fid1 l1 TD lc1 als1 gl Mem1 fs 
+  md m2 flnbep nbs2,
+  validate_metadata_from_module m2 flnbep = true ->
+  flnbeps_to_metadata flnbep = md ->
+  valid_metadata TD fs lc1 Mem1 md = true ->
+  valid_memdata_db TD Mem1 = true ->
+  mtv_cmds Ps1 Ps2 fid1 l1 nbs2 = true ->
+  (exists lc2, exists als2, exists Mem2, exists tr, exists r,
+    SBopsem.dbCmds TD gl lc1 als1 Mem1 (nbranchs2cmds nbs2) lc2 als2 Mem2 tr r 
+    /\
+    valid_metadata TD fs lc2 Mem2 md = true).
+Admitted.
 
 (*****************************)
 (*
